nola/bi/ofe.v
@@ -7,14 +7,7 @@ From iris.base_logic.lib Require Import iprop.
 
 Implicit Type PROP : bi.
 
-Notation oiapp F Σ := (oFunctor_apply F (iProp Σ)).
-Notation riapp F Σ := (rFunctor_apply F (iProp Σ)).
-Module OfeNotation.
-  Notation "F $o Σ" := (oiapp F Σ) (at level 20, right associativity).
-  Notation "F $r Σ" := (riapp F Σ) (at level 20, right associativity).
-End OfeNotation.
-
-(** [▷] on [later PROP] *)
+(** ** [laterl]: [▷] on [later PROP] *)
 Definition laterl {PROP} (P : later PROP) : PROP := ▷ later_car P.
 Arguments laterl {_} _ /.
 
@@ -22,3 +15,11 @@ Arguments laterl {_} _ /.
 #[export] Instance laterl_ne `{!BiLaterContractive PROP} :
   NonExpansive (@laterl PROP).
 Proof. move=> ?[?][?]?/=. by apply later_contractive. Qed.
+
+(** ** Notation for functor application over [iProp Σ] *)
+Notation iProp_oapp F Σ := (oFunctor_apply F (iProp Σ)).
+Notation iProp_rapp F Σ := (rFunctor_apply F (iProp Σ)).
+Module iPropAppNotation.
+  Notation "F $oi Σ" := (iProp_oapp F Σ) (at level 20, right associativity).
+  Notation "F $ri Σ" := (iProp_rapp F Σ) (at level 20, right associativity).
+End iPropAppNotation.
